DS: adapted event/sign preds, added pke preds and adapted third step accordingly
The changes were necessary to get to the point that we can show key secrecy for
the communication key on the responder side. However, the fourth step is not
provable yet because I am not able to show that the event pred holds for the
certify event (within the fourth step).

denning-sacco/DS.Messages.fst
@@ -24,6 +24,8 @@ let parse_sigval_ ssv =
   | t -> Error ("[parse_encsigval] invalid tag: " ^ t)
   ))
 
+let parse_encval_comm_key_ enc_sig_ck = split enc_sig_ck
+
 let serialize_sigval i sv l =
   match sv with
   | CertA a pk_a t ->
@@ -69,9 +71,14 @@ let parse_sigval_lemma ssv = ()
 let parse_serialize_sigval_lemma i sv l = ()
 
 
-let encval_comm_key #i #l ser_ck sig_ck = concat #i #l ser_ck sig_ck
-let parse_encval_comm_key #i #l enc_sig_ck = split #i #l enc_sig_ck
+let encval_comm_key i ser_ck sig_ck l = concat #i #l ser_ck sig_ck
+let parse_encval_comm_key #i #l enc_sig_ck =
+  split #i #l enc_sig_ck `bind` (fun (ser_ck, sig_ck) ->
+  let ser_ck:bytes = ser_ck in
+  let sig_ck:bytes = sig_ck in
+  Success (ser_ck, sig_ck))
 
+let parse_encval_lemma #i #l enc_sig_ck = ()
 let parse_serialize_encval_lemma #i #l ser_ck sig_ck = ()
 
 
