denning-sacco/DS.Messages.fsti
@@ -36,10 +36,23 @@ noeq type sigval =
 val parse_sigval_: ssv:bytes -> result sigval
 
 
+/// Parse decrypted message part, containing the communication key and
+/// a corresponding certificate
+val parse_encval_comm_key_: enc_sig_ck:bytes -> result (ser_ck:bytes * sig_ck:bytes)
+
+
 let ds_key_usages : LC.key_usages = LC.default_key_usages
 
-let can_pke_encrypt (i:nat) s pk m = True (* TODO: Make assumption about label of responders
-secret key in order to infer concrete label of the communication key *)
+let can_pke_encrypt (i:nat) s pk sev =
+  match parse_encval_comm_key_ sev with
+  | Success (ser_ck, _) -> (
+    match parse_sigval_ ser_ck with
+    | Success (CommKey ck t) ->
+      exists a b srv pk_a. was_rand_generated_before i ck (join (readers [P a]) (LC.get_sk_label ds_key_usages pk)) (aead_usage "DS.comm_key") /\
+      (exists clock_cnt. clock_cnt <= recv_msg_2_delay /\ did_event_occur_before i a (event_send_key a b srv pk_a pk ck t clock_cnt))
+    | _ -> False
+  )
+  | _ -> False
 let can_aead_encrypt i s k m ad = True
 let can_sign i s k ssv =
   exists p. LC.get_signkey_label ds_key_usages k == readers [P p] /\
@@ -51,8 +64,8 @@ let can_sign i s k ssv =
     later_than i t /\
     (exists a pk_a. did_event_occur_at t p (event_certify a b p pk_a pk_b t 0))
   | Success (CommKey ck t) ->
-    exists b pk_b. was_rand_generated_before i ck (join (readers [P p]) (LC.get_sk_label ds_key_usages pk_b)) (aead_usage "DS.comm_key") /\
-    (exists srv pk_a clock_cnt. clock_cnt <= recv_msg_2_delay /\ did_event_occur_before i p (event_send_key p b srv pk_a pk_b ck t clock_cnt))
+    exists b srv pk_b. was_rand_generated_before i ck (join (readers [P p]) (LC.get_sk_label ds_key_usages pk_b)) (aead_usage "DS.comm_key") /\
+    (exists clock_cnt. clock_cnt <= recv_msg_2_delay /\ did_event_occur_before i p (event_send_key p b srv k pk_b ck t clock_cnt))
   | _ -> False)
 let can_mac i s k m = True
 
@@ -108,16 +121,31 @@ val parse_serialize_sigval_lemma: i:nat -> sv:sigval -> l:label ->
          SMTPat (parse_sigval_ (serialize_sigval i sv l))]
 
 
+let valid_encval_comm_key (i:nat) (ser_ck sig_ck:bytes) (l:label) =
+  is_msg i ser_ck l /\ is_msg i sig_ck l
+
 /// Create message part to be encrypted, containing the communication key and
 /// a corresponding certificate
-val encval_comm_key: #i:nat -> #l:label -> ser_ck:msg i l -> sig_ck:msg i l -> enc_sig_ck:msg i l
+val encval_comm_key: i:nat -> ser_ck:bytes -> sig_ck:bytes -> l:label{valid_encval_comm_key i ser_ck sig_ck l} -> enc_sig_ck:msg i l
 
 /// Parse decrypted message part, containing the communication key and
 /// a corresponding certificate
-val parse_encval_comm_key: #i:nat -> #l:label -> enc_sig_ck:msg i l -> result (ser_ck:msg i l * sig_ck:msg i l)
+val parse_encval_comm_key: #i:nat -> #l:label -> enc_sig_ck:msg i l -> r:(result (bytes * bytes))
+  {
+    match r with
+    | Success (ser_ck, sig_ck) -> valid_encval_comm_key i ser_ck sig_ck l
+    | _ -> True
+  }
 
-val parse_serialize_encval_lemma: #i:nat -> #l:label -> ser_ck:msg i l -> sig_ck:msg i l ->
-  Lemma (parse_encval_comm_key (encval_comm_key ser_ck sig_ck) == Success (ser_ck, sig_ck))
+val parse_encval_lemma: #i:nat -> #l:label -> enc_sig_ck:msg i l ->
+  Lemma (parse_encval_comm_key enc_sig_ck == parse_encval_comm_key_ enc_sig_ck)
+
+val parse_serialize_encval_lemma: #i:nat -> #l:label -> ser_ck:bytes -> sig_ck:bytes ->
+  Lemma (requires (valid_encval_comm_key i ser_ck sig_ck l))
+        (ensures (parse_encval_comm_key (encval_comm_key i ser_ck sig_ck l) == Success (ser_ck, sig_ck) /\
+                  parse_encval_comm_key_ (encval_comm_key i ser_ck sig_ck l) == Success (ser_ck, sig_ck)))
+        [SMTPat (parse_encval_comm_key (encval_comm_key i ser_ck sig_ck l));
+         SMTPat (parse_encval_comm_key_ (encval_comm_key i ser_ck sig_ck l))]
 
 
 noeq type message (i:nat) =
